\documentclass{beamer}
%\documentclass[aspectratio=169]{beamer}
%
\mode<presentation>
{
  \usetheme{default}      
  \usecolortheme{default}
  \usefonttheme{default} 
  \setbeamertemplate{navigation symbols}{}
  \setbeamertemplate{caption}[numbered]
} 

\usepackage[english]{babel}
\usepackage[utf8x]{inputenc}
\usepackage{amsmath}
\usepackage{bm}
\usepackage{bbm}

\newcommand{\X}{\mathcal{X}}
\newcommand{\Y}{\mathcal{Y}}
\newcommand{\real}{\mathbb{R}}
\newcommand{\N}{\mathbb{N}}
\newcommand{\yhat}{\hat{y}}
\newcommand{\bxi}{\bm{x}^{(i)}}
\newcommand{\bx}{\bm{x}}
\newcommand{\xij}{x^{(i)}_j}
\newcommand{\yi}{y^{(i)}}
\newcommand{\yhati}{\hat{y}^{(i)}}
\newcommand{\norm}[1]{\left\lVert#1\right\rVert}
\newcommand{\1}[1]{\mathbbm{1}\left[#1\right]}

\title[Course presentation]{Machine learning from scratch}
\subtitle{Lecture 2: Convex optimization}
\author{Alexis Zubiolo\newline\texttt{alexis.zubiolo@gmail.com}}
\institute{Data Science Team Lead @ Adcash}
\date{February 2, 2017}

\begin{document}

\begin{frame}
  \titlepage
\end{frame}
\begin{frame}{Optimization: Derivatives}
The \textbf{derivative} is an important concept in optimization and in machine learning. Mathematical definition: Let $f : \real \mapsto \real$ be a function. Its derivative $f'$ is defined by:
\begin{equation*}
	f'(x) = \dfrac{df}{dx}(x) = \lim_{h \to 0}\dfrac{f(x + h) - f(x)}{h}
\end{equation*}
\end{frame}

\begin{frame}{Derivatives: Why we use them (1)}
\textbf{Derivatives} give us an idea of the local behavior of the function.
\vfill
\pause
\textbf{Case 1}: $f'(x) > 0$
\vfill
\pause
Suppose $h > 0$, we have
\begin{equation*}
\begin{split}
f'(x) > 0 & \iff \lim_{h \to 0}\dfrac{f(x + h) - f(x)}{h} > 0 \\
& \iff f(x + h) > f(x) \\
& \iff f \text{ is increasing (because } x + h > x \text{)}
\end{split}
\end{equation*}
\vfill
\pause
Now, suppose $h < 0$, we have
\vfill
\pause
\begin{equation*}
\begin{split}
f'(x) > 0 & \iff \lim_{h \to 0}\dfrac{f(x + h) - f(x)}{h} > 0 \\
& \iff f(x + h) < f(x) \\
& \iff f \text{ is increasing (because } x + h < x \text{)}
\end{split}
\end{equation*}
\vfill
\pause
\textbf{Conclusion}: $f \text{ is increasing} \iff f' > 0$
\end{frame}

\begin{frame}{Derivatives: Why we use them (2)}
\textbf{Case 2}: $f'(x) < 0$
\vfill
\pause
Now, suppose again $h > 0$, we have
\vfill
\pause
\begin{equation*}
\begin{split}
f'(x) > 0 & \iff \lim_{h \to 0}\dfrac{f(x + h) - f(x)}{h} > 0 \\
& \iff f(x + h) < f(x) \\
& \iff f \text{ is increasing}
\end{split}
\end{equation*}
\pause
\vfill
\pause
Suppose again $h < 0$, we have:
\vfill
\pause
\begin{equation*}
\begin{split}
\lim_{h \to 0}\dfrac{f(x + h) - f(x)}{h} < 0 & \iff f(x + h) - f(x) = 0 \\
 & \iff f(x + h) = f(x)
\end{split}
\end{equation*}
\vfill
\pause
\textbf{Conclusion}: $f \text{ is decreasing} \iff f' < 0$
\end{frame}

\begin{frame}{Derivatives: Why we use them (3)}
\textbf{Case 3}: $f'(x) = 0$, then 
\vfill
\pause
\begin{equation*}
\begin{split}
f'(x) = 0 & \iff \lim_{h \to 0}\dfrac{f(x + h) - f(x)}{h} = 0 \\
& \iff f(x + h) = f(x) \\
& \iff f \text{ is constant}
\end{split}
\end{equation*}
\vfill
\pause
\textbf{Conclusion}: $f$ is constant $\iff f = 0$
\vfill
\pause
\textbf{Summary}:
\begin{itemize}
	\item $f \text{ is increasing} \iff f'(x) > 0$
	\item $f \text{ is decreasing} \iff f'(x) < 0$
	\item $f \text{ is constant} \iff f'(x) = 0$
\end{itemize}
\end{frame}

\begin{frame}{Derivatives: Why we use them (4)}
\textbf{Summary}:
\begin{itemize}
	\item $f \text{ is increasing} \iff f'(x) > 0$
	\item $f \text{ is decreasing} \iff f'(x) < 0$
	\item $f \text{ is constant} \iff f'(x) = 0$
\end{itemize}
\vfill
\pause
What do we do with this?
\vfill
\pause
If we want to find $f$'s minimum, a strategy could be:
\begin{enumerate}
	\item Start at a random point $x_0 \in \real$
	\item Compute $f'(x_0)$ and then
	\begin{itemize}
		\item if $f'(x_0) > 0$ then move to the left (because $f$ is increasing) 
		\item if $f'(x_0) < 0$ then move to the right (because $f$ is decreasing)
		\item if $f'(x_0) = 0$ then we stop
	\end{itemize}
\end{enumerate}
\end{frame}

\begin{frame}{Derivatives: How to compute them?}
There are several ways to compute the derivatives.
\begin{itemize}
\vfill
\pause
	\item By \textbf{applying the definition}
\begin{equation*}
	f'(x) = \dfrac{df}{dx}(x) = \lim_{h \to 0}\dfrac{f(x + h) - f(x)}{h}
\end{equation*}
	with a small $h$ (\textit{e.g.} $h = 0.01$). This is called the \textbf{finite difference approximation}.
	\item By using \textbf{closed-form derivatives}, \textit{e.g.}
\begin{equation*}
	\text{if } f(x) = x^2 \text{, then } f'(x) = 2x
\end{equation*}
	How do we know that? By using the formula!
\end{itemize}
\end{frame}

\begin{frame}{Derivative: Practical example}
Recall the definition:
\begin{equation*}
\begin{split}
	f'(x) &= \lim_{h \to 0}\dfrac{f(x + h) - f(x)}{h}
\end{split}
\end{equation*}
\textbf{Exercice}: Apply this formula for $f(x) = x^2$. What is $f'(x)$?
\pause
\vfill
\begin{equation*}
\begin{split}
	f'(x) &= \lim_{h \to 0}\dfrac{(x + h)^2 - x^2}{h} \\
	& = \lim_{h \to 0}\dfrac{x^2 + 2hx + h^2 - x^2}{h} \\
	& = \lim_{h \to 0}\dfrac{2hx + h^2}{h} \\
	& = \lim_{h \to 0} 2x + h = 2x
\end{split}
\end{equation*}
We can apply this logic to the usual functions ($\log$, $\cos$, $\sin$, \ldots) and obtain what we call \textbf{closed-form solutions}. 
\vfill
\pause
\textbf{Exercise}: Do the same for $f(x) = \frac{1}{x}$.
\end{frame}

\begin{frame}{Derivatives: Finite difference approximation}
\textbf{Recall}: The \textbf{finite difference approximation} consists in applying the following formula
\begin{equation*}
	f'(x) = \dfrac{df}{dx}(x) = \lim_{h \to 0}\dfrac{f(x + h) - f(x)}{h}
\end{equation*}
with $h$ close enough to $0$.
\pause
\vfill
There's a symmetric and more stable formula, called the \textbf{centered finite difference approximation}.
\begin{equation*}
	f'(x) = \dfrac{df}{dx}(x) = \lim_{h \to 0}\dfrac{f(x + h) - f(x - h)}{2h}
\end{equation*}
\end{frame}

\begin{frame}{Chain rule}
Another important rule concerning derivatives is the \textbf{chain rule}:
\begin{equation}
	(f(g(x)))' = g'(x) f'(g(x))
\end{equation}
or, equivalently:
\begin{equation}
	\dfrac{df(g(x))}{dx} = \dfrac{df(g)}{dg} \dfrac{dg(x)}{dx}
\end{equation}
\end{frame}

\begin{frame}{Gradient: Generalizing the derivatives}
Derivatives look like a practical way to get the minimum of a function, which is what we want to achieve (minimizing $J(\theta)$).
\vfill
\pause
However, the definition we've seen only applies to function from $\real$ to $\real$. The \textbf{gradient} is a generalization of the derivative for functions from $\real^d$ to $\real$, like $J$.
\end{frame}

\begin{frame}{Beyond derivatives: Gradient}
Let's consider a function of $f$ 2 real variables $x$ and $y$, \textit{e.g.}
\begin{equation*}
f(x, y) = xy
\end{equation*}
The gradient of $f$ is a 2-dimensional vector noted $\nabla f$ defined by:
\begin{equation*}
\nabla f(x, y) = \left[ \dfrac{\partial f(x, y)}{\partial x}, \dfrac{\partial f(x, y)}{\partial y} \right]
\end{equation*}
where 
$$\dfrac{\partial f(x, y)}{\partial x}$$ 
is the \textbf{partial derivative} of $f$ with respect to $x$ (considering $y$ as a constant), and 
$$\dfrac{\partial f(x, y)}{\partial x}$$ 
is the \textbf{partial derivative} of $f$ with respect to $y$ (considering $x$ as a constant).
\vfill
\pause
\textbf{Exercise}: What is $\nabla f(x, y)$ for $f(x, y) = xy$ and $f(x, y) = x + y$?
\end{frame}

\begin{frame}{Beyond derivatives: Gradient}
Interpretation of the gradient: Direction of \textbf{steepest descent} of $f$
\end{frame}

\begin{frame}{Back to least squares: context reminder}
\begin{table}
\centering
\begin{tabular}{r|r|r|r}
living area (m$^2$) & \# bedrooms & intercept & price (1000's BGN) \\\hline
50 & 1 & 1 & 30\\
76 & 2 & 1 & 48\\
26 & 1 & 1 & 12\\
102 & 3 & 1 & 90\\
\end{tabular}
\end{table}
\vfill
\begin{equation*}
h(\bx) = \sum_{j = 0}^{d} \theta_j x_j = \theta^T \bx
\end{equation*}
\pause
\vfill
Suppose we chose the following loss function:
\begin{equation*}
\ell \left( y, \yhat \right) = \dfrac{1}{2} \left( y - \yhat \right)^2
\end{equation*}
This leads to the following least squares \textit{cost function}:
\begin{equation*}
J(\theta) = \dfrac{1}{2} \sum_{i = 1}^{n} \left( h\left(\bxi\right) - \yi \right)^2
\end{equation*}
This problem the \textbf{ordinary least squares} (OLS) regression model.
\end{frame}

\begin{frame}{Least Mean Squares (LMS) update rule}
To apply the LMS update rule, we need to compute the gradient of $J$. Let's compute it for a single $(\bx, y)$ sample:
\begin{equation*}
\begin{split}
\dfrac{\partial}{\partial \theta_j} J(\theta) & = \dfrac{\partial}{\partial \theta_j} \dfrac{1}{2} \left( h\left(\bx\right) - y \right)^2 \\ 
 & = \text{?} \\
\end{split}
\end{equation*}
where $h(\bx) = \sum_{j = 0}^{d} \theta_j x_j = \theta^T \bx$
\vfill
\pause
\textbf{Exercise}: Compute the gradient and find the update rule.
\end{frame}

\begin{frame}{Least Mean Squares (LMS) update rule}
\textbf{Solution}: 
\begin{equation*}
\begin{split}
\dfrac{\partial}{\partial \theta_j} J(\theta) & = \dfrac{\partial}{\partial \theta_j} \dfrac{1}{2} \left( h\left(\bx\right) - y \right)^2 \\ 
 & = 2 \dfrac{1}{2} \left( h\left(\bx\right) - y \right) \dfrac{\partial}{\partial \theta_j}\left( h\left(\bx\right) - y \right)\\
 & = \left( h\left(\bx\right) - y \right) \dfrac{\partial}{\partial \theta_j}\left( \sum_{k = 0}^{d} \theta_k x_k - y \right)\\
 & = \left( h\left(\bx\right) - y \right) x_j\\
\end{split}
\end{equation*}
\pause
\vfill
So the gradient descent update becomes
\begin{equation*}
\begin{split}
\theta_j &:= \theta_j - \alpha \dfrac{\partial}{\partial \theta_j} J(\theta) \\
 & := \theta_j + \alpha \left( y - h\left(\bx\right)\right) x_j
\end{split}
\end{equation*}
\end{frame}

\begin{frame}{Conclusion}
We had an overview of the optimization techniques. 
\vfill
\pause
Next Thursday, we will review what needs to be reviewed (tell me by email so that I can adapt or when the class starts) and start implementing:
\begin{itemize}
	\item The loss function for the least-squares problem
	\item Its gradient
	\item The Gradient descent weight upgrade
	\item Run it on a toy example
\end{itemize}
\end{frame}

\begin{frame}
\vfill
\centering
\begin{huge}
\huge{Thank you! Questions?}
\vfill
\texttt{alexis.zubiolo@gmail.com}
\end{huge}
\vfill
\begin{Large}
\texttt{https://github.com/azubiolo/itstep}
\end{Large}
\vfill
\end{frame}

\end{document}
